compiler/dafny/vcg/dafny_wp_calcScript.sml
@@ -1307,7 +1307,7 @@ Theorem Rcont_eval_measure[local]:
   eval_measure st env (wrap_old decs)
 Proof
   strip_tac
-  \\ imp_res_tac eval_stmt_Rcont_const
+  \\ imp_res_tac eval_stmt_const
   \\ namedCases_on ‘decs’ ["rank es"]
   \\ simp [wrap_old_def, eval_measure_def]
   \\ DEP_REWRITE_TAC [eval_decreases_old_eq]
